extraction of let mut

pulse/pulse2rust/src/ocaml/generated/Pulse2Rust.ml
@@ -1,4 +1,15 @@
 open Prims
+type var = Prims.string
+type binding = (var * Pulse2Rust_Rust_Syntax.typ * Prims.bool)
+type env =
+  {
+  fvs: (Prims.string * Pulse2Rust_Rust_Syntax.fn_signature) Prims.list ;
+  gamma: binding Prims.list }
+let (__proj__Mkenv__item__fvs :
+  env -> (Prims.string * Pulse2Rust_Rust_Syntax.fn_signature) Prims.list) =
+  fun projectee -> match projectee with | { fvs; gamma;_} -> fvs
+let (__proj__Mkenv__item__gamma : env -> binding Prims.list) =
+  fun projectee -> match projectee with | { fvs; gamma;_} -> gamma
 let (tyvar_of : Prims.string -> Prims.string) =
   fun s ->
     let uu___ =
@@ -18,6 +29,63 @@ let fail_nyi : 'uuuuu . Prims.string -> 'uuuuu =
       FStar_Compiler_Util.format1
         "Pulse to Rust extraction failed: no support yet for %s" s in
     failwith uu___
+let (empty_env : unit -> env) = fun uu___ -> { fvs = []; gamma = [] }
+let (lookup_global_fn :
+  env ->
+    Prims.string ->
+      Pulse2Rust_Rust_Syntax.fn_signature FStar_Pervasives_Native.option)
+  =
+  fun g ->
+    fun s ->
+      let uu___ =
+        FStar_Compiler_List.tryFind
+          (fun uu___1 -> match uu___1 with | (f, uu___2) -> f = s) g.fvs in
+      FStar_Compiler_Util.map_option
+        (fun uu___1 -> match uu___1 with | (uu___2, t) -> t) uu___
+let (lookup_local :
+  env ->
+    Prims.string ->
+      (Pulse2Rust_Rust_Syntax.typ * Prims.bool)
+        FStar_Pervasives_Native.option)
+  =
+  fun g ->
+    fun s ->
+      let uu___ =
+        FStar_Compiler_List.tryFind
+          (fun uu___1 -> match uu___1 with | (x, uu___2, uu___3) -> x = s)
+          g.gamma in
+      FStar_Compiler_Util.map_option
+        (fun uu___1 -> match uu___1 with | (uu___2, t, b) -> (t, b)) uu___
+let (push_fv :
+  env -> Prims.string -> Pulse2Rust_Rust_Syntax.fn_signature -> env) =
+  fun g -> fun s -> fun t -> { fvs = ((s, t) :: (g.fvs)); gamma = (g.gamma) }
+let (push_local :
+  env -> Prims.string -> Pulse2Rust_Rust_Syntax.typ -> Prims.bool -> env) =
+  fun g ->
+    fun s ->
+      fun t ->
+        fun is_mut ->
+          { fvs = (g.fvs); gamma = ((s, t, is_mut) :: (g.gamma)) }
+let (type_of :
+  env ->
+    Pulse2Rust_Rust_Syntax.expr -> (Pulse2Rust_Rust_Syntax.typ * Prims.bool))
+  =
+  fun g ->
+    fun e ->
+      match e with
+      | Pulse2Rust_Rust_Syntax.Expr_path s ->
+          let uu___ = lookup_local g s in
+          (match uu___ with
+           | FStar_Pervasives_Native.Some (t, b) -> (t, b)
+           | FStar_Pervasives_Native.None ->
+               let uu___1 =
+                 FStar_Compiler_Util.format1 "lookup in env for %s" s in
+               fail uu___1)
+      | uu___ ->
+          let uu___1 =
+            let uu___2 = RustBindings.expr_to_string e in
+            FStar_Compiler_Util.format1 "type_of %s" uu___2 in
+          fail_nyi uu___1
 let rec (uncurry_arrow :
   FStar_Extraction_ML_Syntax.mlty ->
     (FStar_Extraction_ML_Syntax.mlty Prims.list *
@@ -29,95 +97,133 @@ let rec (uncurry_arrow :
         let uu___1 = uncurry_arrow t2 in
         (match uu___1 with | (arg_ts, ret_t) -> ((t1 :: arg_ts), ret_t))
     | uu___ -> ([], t)
-let (extract_mlty :
-  FStar_Extraction_ML_Syntax.mlty -> Pulse2Rust_Rust_Syntax.typ) =
-  fun t ->
-    match t with
-    | FStar_Extraction_ML_Syntax.MLTY_Var s ->
-        let uu___ = tyvar_of s in Pulse2Rust_Rust_Syntax.Typ_name uu___
-    | FStar_Extraction_ML_Syntax.MLTY_Named ([], p) when
-        let uu___ = FStar_Extraction_ML_Syntax.string_of_mlpath p in
-        uu___ = "FStar.UInt32.t" -> Pulse2Rust_Rust_Syntax.Typ_name "u32"
-    | FStar_Extraction_ML_Syntax.MLTY_Named ([], p) when
-        let uu___ = FStar_Extraction_ML_Syntax.string_of_mlpath p in
-        uu___ = "FStar.Int32.t" -> Pulse2Rust_Rust_Syntax.Typ_name "i32"
-    | FStar_Extraction_ML_Syntax.MLTY_Named ([], p) when
-        let uu___ = FStar_Extraction_ML_Syntax.string_of_mlpath p in
-        uu___ = "FStar.UInt64.t" -> Pulse2Rust_Rust_Syntax.Typ_name "u64"
-    | FStar_Extraction_ML_Syntax.MLTY_Named ([], p) when
-        let uu___ = FStar_Extraction_ML_Syntax.string_of_mlpath p in
-        uu___ = "FStar.Int64.t" -> Pulse2Rust_Rust_Syntax.Typ_name "i64"
-    | FStar_Extraction_ML_Syntax.MLTY_Named ([], p) when
-        let uu___ = FStar_Extraction_ML_Syntax.string_of_mlpath p in
-        uu___ = "Prims.bool" -> Pulse2Rust_Rust_Syntax.Typ_name "bool"
-    | FStar_Extraction_ML_Syntax.MLTY_Erased ->
-        Pulse2Rust_Rust_Syntax.Typ_name "unit"
-    | uu___ ->
-        let uu___1 =
-          let uu___2 = FStar_Extraction_ML_Syntax.mlty_to_string t in
-          FStar_Compiler_Util.format1 "mlty %s" uu___2 in
-        fail_nyi uu___1
-let (extract_top_level_fn_arg :
-  Prims.string ->
-    FStar_Extraction_ML_Syntax.mlty -> Pulse2Rust_Rust_Syntax.fn_arg)
-  =
-  fun arg_name ->
+let rec (extract_mlty :
+  env -> FStar_Extraction_ML_Syntax.mlty -> Pulse2Rust_Rust_Syntax.typ) =
+  fun g ->
     fun t ->
       match t with
       | FStar_Extraction_ML_Syntax.MLTY_Var s ->
-          let uu___ =
-            let uu___1 = tyvar_of s in Pulse2Rust_Rust_Syntax.Typ_name uu___1 in
-          Pulse2Rust_Rust_Syntax.mk_scalar_fn_arg arg_name uu___
+          let uu___ = tyvar_of s in Pulse2Rust_Rust_Syntax.Typ_name uu___
       | FStar_Extraction_ML_Syntax.MLTY_Named ([], p) when
-          ((((let uu___ = FStar_Extraction_ML_Syntax.string_of_mlpath p in
-              uu___ = "FStar.UInt32.t") ||
-               (let uu___ = FStar_Extraction_ML_Syntax.string_of_mlpath p in
-                uu___ = "FStar.Int32.t"))
-              ||
-              (let uu___ = FStar_Extraction_ML_Syntax.string_of_mlpath p in
-               uu___ = "FStar.UInt64.t"))
-             ||
-             (let uu___ = FStar_Extraction_ML_Syntax.string_of_mlpath p in
-              uu___ = "FStar.Int64.t"))
-            ||
+          let uu___ = FStar_Extraction_ML_Syntax.string_of_mlpath p in
+          uu___ = "FStar.UInt32.t" -> Pulse2Rust_Rust_Syntax.Typ_name "u32"
+      | FStar_Extraction_ML_Syntax.MLTY_Named ([], p) when
+          let uu___ = FStar_Extraction_ML_Syntax.string_of_mlpath p in
+          uu___ = "FStar.Int32.t" -> Pulse2Rust_Rust_Syntax.Typ_name "i32"
+      | FStar_Extraction_ML_Syntax.MLTY_Named ([], p) when
+          let uu___ = FStar_Extraction_ML_Syntax.string_of_mlpath p in
+          uu___ = "FStar.UInt64.t" -> Pulse2Rust_Rust_Syntax.Typ_name "u64"
+      | FStar_Extraction_ML_Syntax.MLTY_Named ([], p) when
+          (let uu___ = FStar_Extraction_ML_Syntax.string_of_mlpath p in
+           uu___ = "FStar.Int64.t") ||
             (let uu___ = FStar_Extraction_ML_Syntax.string_of_mlpath p in
-             uu___ = "Prims.bool")
-          ->
-          let uu___ = extract_mlty t in
-          Pulse2Rust_Rust_Syntax.mk_scalar_fn_arg arg_name uu___
+             uu___ = "Prims.int")
+          -> Pulse2Rust_Rust_Syntax.Typ_name "i64"
+      | FStar_Extraction_ML_Syntax.MLTY_Named ([], p) when
+          let uu___ = FStar_Extraction_ML_Syntax.string_of_mlpath p in
+          uu___ = "Prims.bool" -> Pulse2Rust_Rust_Syntax.Typ_name "bool"
       | FStar_Extraction_ML_Syntax.MLTY_Named (arg::[], p) when
           let uu___ = FStar_Extraction_ML_Syntax.string_of_mlpath p in
           uu___ = "Pulse.Lib.Reference.ref" ->
           let is_mut = true in
-          let uu___ = extract_mlty arg in
-          Pulse2Rust_Rust_Syntax.mk_ref_fn_arg arg_name is_mut uu___
+          let uu___ = extract_mlty g arg in
+          Pulse2Rust_Rust_Syntax.mk_ref_typ is_mut uu___
       | FStar_Extraction_ML_Syntax.MLTY_Erased ->
-          Pulse2Rust_Rust_Syntax.mk_scalar_fn_arg arg_name
-            (Pulse2Rust_Rust_Syntax.Typ_name "unit")
+          Pulse2Rust_Rust_Syntax.Typ_name "unit"
       | uu___ ->
           let uu___1 =
             let uu___2 = FStar_Extraction_ML_Syntax.mlty_to_string t in
-            FStar_Compiler_Util.format1 "top level fn arg %s" uu___2 in
+            FStar_Compiler_Util.format1 "mlty %s" uu___2 in
           fail_nyi uu___1
-let (extract_top_level_sig :
-  Prims.string ->
-    FStar_Extraction_ML_Syntax.mlidents ->
-      Prims.string Prims.list ->
-        FStar_Extraction_ML_Syntax.mlty Prims.list ->
-          FStar_Extraction_ML_Syntax.mlty ->
-            Pulse2Rust_Rust_Syntax.fn_signature)
+let (extract_top_level_fn_arg :
+  env ->
+    Prims.string ->
+      FStar_Extraction_ML_Syntax.mlty -> Pulse2Rust_Rust_Syntax.fn_arg)
   =
-  fun fn_name ->
-    fun tvars ->
-      fun arg_names ->
-        fun arg_ts ->
-          fun ret_t ->
-            let fn_args =
-              let uu___ = FStar_Compiler_List.map varname arg_names in
-              FStar_Compiler_List.map2 extract_top_level_fn_arg uu___ arg_ts in
-            let fn_ret_t = extract_mlty ret_t in
-            Pulse2Rust_Rust_Syntax.mk_fn_signature fn_name tvars fn_args
-              fn_ret_t
+  fun g ->
+    fun arg_name ->
+      fun t ->
+        match t with
+        | FStar_Extraction_ML_Syntax.MLTY_Var s ->
+            let uu___ =
+              let uu___1 = tyvar_of s in
+              Pulse2Rust_Rust_Syntax.Typ_name uu___1 in
+            Pulse2Rust_Rust_Syntax.mk_scalar_fn_arg arg_name uu___
+        | FStar_Extraction_ML_Syntax.MLTY_Named ([], p) when
+            (((((let uu___ = FStar_Extraction_ML_Syntax.string_of_mlpath p in
+                 uu___ = "FStar.UInt32.t") ||
+                  (let uu___ = FStar_Extraction_ML_Syntax.string_of_mlpath p in
+                   uu___ = "FStar.Int32.t"))
+                 ||
+                 (let uu___ = FStar_Extraction_ML_Syntax.string_of_mlpath p in
+                  uu___ = "FStar.UInt64.t"))
+                ||
+                (let uu___ = FStar_Extraction_ML_Syntax.string_of_mlpath p in
+                 uu___ = "FStar.Int64.t"))
+               ||
+               (let uu___ = FStar_Extraction_ML_Syntax.string_of_mlpath p in
+                uu___ = "Prims.int"))
+              ||
+              (let uu___ = FStar_Extraction_ML_Syntax.string_of_mlpath p in
+               uu___ = "Prims.bool")
+            ->
+            let uu___ = extract_mlty g t in
+            Pulse2Rust_Rust_Syntax.mk_scalar_fn_arg arg_name uu___
+        | FStar_Extraction_ML_Syntax.MLTY_Named (arg::[], p) when
+            let uu___ = FStar_Extraction_ML_Syntax.string_of_mlpath p in
+            uu___ = "Pulse.Lib.Reference.ref" ->
+            let uu___ = extract_mlty g t in
+            Pulse2Rust_Rust_Syntax.mk_scalar_fn_arg arg_name uu___
+        | FStar_Extraction_ML_Syntax.MLTY_Erased ->
+            Pulse2Rust_Rust_Syntax.mk_scalar_fn_arg arg_name
+              (Pulse2Rust_Rust_Syntax.Typ_name "unit")
+        | uu___ ->
+            let uu___1 =
+              let uu___2 = FStar_Extraction_ML_Syntax.mlty_to_string t in
+              FStar_Compiler_Util.format1 "top level fn arg %s" uu___2 in
+            fail_nyi uu___1
+let (push_fn_arg :
+  env -> Prims.string -> Pulse2Rust_Rust_Syntax.fn_arg -> env) =
+  fun g ->
+    fun arg_name ->
+      fun arg ->
+        match arg with
+        | Pulse2Rust_Rust_Syntax.Fn_arg_pat
+            { Pulse2Rust_Rust_Syntax.pat_typ_pat = uu___;
+              Pulse2Rust_Rust_Syntax.pat_typ_typ = pat_typ_typ;_}
+            -> let is_mut = false in push_local g arg_name pat_typ_typ false
+let (extract_top_level_sig :
+  env ->
+    Prims.string ->
+      FStar_Extraction_ML_Syntax.mlidents ->
+        Prims.string Prims.list ->
+          FStar_Extraction_ML_Syntax.mlty Prims.list ->
+            FStar_Extraction_ML_Syntax.mlty ->
+              (Pulse2Rust_Rust_Syntax.fn_signature * env))
+  =
+  fun g ->
+    fun fn_name ->
+      fun tvars ->
+        fun arg_names ->
+          fun arg_ts ->
+            fun ret_t ->
+              let fn_args =
+                let uu___ = FStar_Compiler_List.map varname arg_names in
+                FStar_Compiler_List.map2 (extract_top_level_fn_arg g) uu___
+                  arg_ts in
+              let fn_ret_t = extract_mlty g ret_t in
+              let uu___ =
+                Pulse2Rust_Rust_Syntax.mk_fn_signature fn_name tvars fn_args
+                  fn_ret_t in
+              let uu___1 =
+                let uu___2 = FStar_Compiler_List.zip arg_names fn_args in
+                FStar_Compiler_List.fold_left
+                  (fun g1 ->
+                     fun uu___3 ->
+                       match uu___3 with
+                       | (arg_name, arg) -> push_fn_arg g1 arg_name arg) g
+                  uu___2 in
+              (uu___, uu___1)
 let (arg_ts_and_ret_t :
   FStar_Extraction_ML_Syntax.mltyscheme ->
     (FStar_Extraction_ML_Syntax.mlidents * FStar_Extraction_ML_Syntax.mlty
@@ -143,225 +249,317 @@ let (arg_ts_and_ret_t :
                  uu___3 in
              fail_nyi uu___2)
 let rec (extract_mlexpr :
-  FStar_Extraction_ML_Syntax.mlexpr -> Pulse2Rust_Rust_Syntax.expr) =
-  fun e ->
-    match e.FStar_Extraction_ML_Syntax.expr with
-    | FStar_Extraction_ML_Syntax.MLE_Const
-        (FStar_Extraction_ML_Syntax.MLC_Unit) ->
-        Pulse2Rust_Rust_Syntax.Expr_path "unitv"
-    | FStar_Extraction_ML_Syntax.MLE_Const
-        (FStar_Extraction_ML_Syntax.MLC_Int (lit_int_val, swopt)) ->
-        let lit_int_signed =
-          match swopt with
-          | FStar_Pervasives_Native.Some (FStar_Const.Unsigned, uu___) ->
-              FStar_Pervasives_Native.Some false
-          | FStar_Pervasives_Native.Some (FStar_Const.Signed, uu___) ->
-              FStar_Pervasives_Native.Some true
-          | FStar_Pervasives_Native.None -> FStar_Pervasives_Native.None in
-        let lit_int_width =
-          match swopt with
-          | FStar_Pervasives_Native.Some (uu___, FStar_Const.Int8) ->
-              FStar_Pervasives_Native.Some Pulse2Rust_Rust_Syntax.I8
-          | FStar_Pervasives_Native.Some (uu___, FStar_Const.Int16) ->
-              FStar_Pervasives_Native.Some Pulse2Rust_Rust_Syntax.I16
-          | FStar_Pervasives_Native.Some (uu___, FStar_Const.Int32) ->
-              FStar_Pervasives_Native.Some Pulse2Rust_Rust_Syntax.I32
-          | FStar_Pervasives_Native.Some (uu___, FStar_Const.Int64) ->
-              FStar_Pervasives_Native.Some Pulse2Rust_Rust_Syntax.I64
-          | FStar_Pervasives_Native.None -> FStar_Pervasives_Native.None in
-        Pulse2Rust_Rust_Syntax.Expr_lit
-          (Pulse2Rust_Rust_Syntax.Lit_int
-             {
-               Pulse2Rust_Rust_Syntax.lit_int_val = lit_int_val;
-               Pulse2Rust_Rust_Syntax.lit_int_signed = lit_int_signed;
-               Pulse2Rust_Rust_Syntax.lit_int_width = lit_int_width
-             })
-    | FStar_Extraction_ML_Syntax.MLE_Var x ->
-        let uu___ = varname x in Pulse2Rust_Rust_Syntax.Expr_path uu___
-    | FStar_Extraction_ML_Syntax.MLE_Name p ->
-        Pulse2Rust_Rust_Syntax.Expr_path (FStar_Pervasives_Native.snd p)
-    | FStar_Extraction_ML_Syntax.MLE_Let uu___ ->
-        let uu___1 =
-          FStar_Compiler_Effect.op_Bar_Greater e extract_mlexpr_to_stmts in
-        FStar_Compiler_Effect.op_Bar_Greater uu___1
-          Pulse2Rust_Rust_Syntax.mk_block_expr
-    | FStar_Extraction_ML_Syntax.MLE_App
-        ({
-           FStar_Extraction_ML_Syntax.expr =
-             FStar_Extraction_ML_Syntax.MLE_TApp
-             ({
-                FStar_Extraction_ML_Syntax.expr =
-                  FStar_Extraction_ML_Syntax.MLE_Name p;
-                FStar_Extraction_ML_Syntax.mlty = uu___;
-                FStar_Extraction_ML_Syntax.loc = uu___1;_},
-              uu___2::[]);
-           FStar_Extraction_ML_Syntax.mlty = uu___3;
-           FStar_Extraction_ML_Syntax.loc = uu___4;_},
-         e1::e2::uu___5::[])
-        when
-        let uu___6 = FStar_Extraction_ML_Syntax.string_of_mlpath p in
-        uu___6 = "Pulse.Lib.Reference.op_Colon_Equals" ->
-        let e11 = extract_mlexpr e1 in
-        let e21 = extract_mlexpr e2 in
-        Pulse2Rust_Rust_Syntax.mk_ref_assign e11 e21
-    | FStar_Extraction_ML_Syntax.MLE_App
-        ({
-           FStar_Extraction_ML_Syntax.expr =
-             FStar_Extraction_ML_Syntax.MLE_TApp
-             ({
-                FStar_Extraction_ML_Syntax.expr =
-                  FStar_Extraction_ML_Syntax.MLE_Name p;
-                FStar_Extraction_ML_Syntax.mlty = uu___;
-                FStar_Extraction_ML_Syntax.loc = uu___1;_},
-              uu___2::[]);
-           FStar_Extraction_ML_Syntax.mlty = uu___3;
-           FStar_Extraction_ML_Syntax.loc = uu___4;_},
-         e1::uu___5::uu___6::[])
-        when
-        let uu___7 = FStar_Extraction_ML_Syntax.string_of_mlpath p in
-        uu___7 = "Pulse.Lib.Reference.op_Bang" ->
-        let e2 = extract_mlexpr e1 in Pulse2Rust_Rust_Syntax.mk_ref_read e2
-    | FStar_Extraction_ML_Syntax.MLE_App
-        ({
-           FStar_Extraction_ML_Syntax.expr =
-             FStar_Extraction_ML_Syntax.MLE_Name p;
-           FStar_Extraction_ML_Syntax.mlty = uu___;
-           FStar_Extraction_ML_Syntax.loc = uu___1;_},
-         {
-           FStar_Extraction_ML_Syntax.expr =
-             FStar_Extraction_ML_Syntax.MLE_Fun (uu___2, cond);
-           FStar_Extraction_ML_Syntax.mlty = uu___3;
-           FStar_Extraction_ML_Syntax.loc = uu___4;_}::{
-                                                         FStar_Extraction_ML_Syntax.expr
-                                                           =
-                                                           FStar_Extraction_ML_Syntax.MLE_Fun
-                                                           (uu___5, body);
-                                                         FStar_Extraction_ML_Syntax.mlty
-                                                           = uu___6;
-                                                         FStar_Extraction_ML_Syntax.loc
-                                                           = uu___7;_}::[])
-        when
-        let uu___8 = FStar_Extraction_ML_Syntax.string_of_mlpath p in
-        uu___8 = "Pulse.Lib.Core.while_" ->
-        let expr_while_cond = extract_mlexpr cond in
-        let expr_while_body = extract_mlexpr_to_stmts body in
-        Pulse2Rust_Rust_Syntax.Expr_while
-          {
-            Pulse2Rust_Rust_Syntax.expr_while_cond = expr_while_cond;
-            Pulse2Rust_Rust_Syntax.expr_while_body = expr_while_body
-          }
-    | FStar_Extraction_ML_Syntax.MLE_App (head, args) ->
-        let head1 = extract_mlexpr head in
-        let args1 = FStar_Compiler_List.map extract_mlexpr args in
-        Pulse2Rust_Rust_Syntax.mk_call head1 args1
-    | FStar_Extraction_ML_Syntax.MLE_TApp (head, uu___) ->
-        extract_mlexpr head
-    | FStar_Extraction_ML_Syntax.MLE_If (cond, if_then, if_else_opt) ->
-        let cond1 = extract_mlexpr cond in
-        let then_ = extract_mlexpr_to_stmts if_then in
-        let else_ = FStar_Compiler_Util.map_option extract_mlexpr if_else_opt in
-        let else_1 =
-          match else_ with
-          | FStar_Pervasives_Native.None -> else_
-          | FStar_Pervasives_Native.Some (Pulse2Rust_Rust_Syntax.Expr_if
-              uu___) -> else_
-          | FStar_Pervasives_Native.Some (Pulse2Rust_Rust_Syntax.Expr_block
-              uu___) -> else_
-          | FStar_Pervasives_Native.Some else_2 ->
-              let uu___ =
-                Pulse2Rust_Rust_Syntax.mk_block_expr
-                  [Pulse2Rust_Rust_Syntax.Stmt_expr else_2] in
-              FStar_Pervasives_Native.Some uu___ in
-        Pulse2Rust_Rust_Syntax.mk_if cond1 then_ else_1
-    | uu___ ->
-        let uu___1 =
-          let uu___2 = FStar_Extraction_ML_Syntax.mlexpr_to_string e in
-          FStar_Compiler_Util.format1 "mlexpr %s" uu___2 in
-        fail_nyi uu___1
-and (extract_mlexpr_to_stmts :
-  FStar_Extraction_ML_Syntax.mlexpr -> Pulse2Rust_Rust_Syntax.stmt Prims.list)
-  =
-  fun e ->
-    match e.FStar_Extraction_ML_Syntax.expr with
-    | FStar_Extraction_ML_Syntax.MLE_Const
-        (FStar_Extraction_ML_Syntax.MLC_Unit) -> []
-    | FStar_Extraction_ML_Syntax.MLE_Var x ->
-        let uu___ =
+  env -> FStar_Extraction_ML_Syntax.mlexpr -> Pulse2Rust_Rust_Syntax.expr) =
+  fun g ->
+    fun e ->
+      match e.FStar_Extraction_ML_Syntax.expr with
+      | FStar_Extraction_ML_Syntax.MLE_Const
+          (FStar_Extraction_ML_Syntax.MLC_Unit) ->
+          Pulse2Rust_Rust_Syntax.Expr_path "unitv"
+      | FStar_Extraction_ML_Syntax.MLE_Const
+          (FStar_Extraction_ML_Syntax.MLC_Int (lit_int_val, swopt)) ->
+          let lit_int_signed =
+            match swopt with
+            | FStar_Pervasives_Native.Some (FStar_Const.Unsigned, uu___) ->
+                FStar_Pervasives_Native.Some false
+            | FStar_Pervasives_Native.Some (FStar_Const.Signed, uu___) ->
+                FStar_Pervasives_Native.Some true
+            | FStar_Pervasives_Native.None -> FStar_Pervasives_Native.None in
+          let lit_int_width =
+            match swopt with
+            | FStar_Pervasives_Native.Some (uu___, FStar_Const.Int8) ->
+                FStar_Pervasives_Native.Some Pulse2Rust_Rust_Syntax.I8
+            | FStar_Pervasives_Native.Some (uu___, FStar_Const.Int16) ->
+                FStar_Pervasives_Native.Some Pulse2Rust_Rust_Syntax.I16
+            | FStar_Pervasives_Native.Some (uu___, FStar_Const.Int32) ->
+                FStar_Pervasives_Native.Some Pulse2Rust_Rust_Syntax.I32
+            | FStar_Pervasives_Native.Some (uu___, FStar_Const.Int64) ->
+                FStar_Pervasives_Native.Some Pulse2Rust_Rust_Syntax.I64
+            | FStar_Pervasives_Native.None -> FStar_Pervasives_Native.None in
+          Pulse2Rust_Rust_Syntax.Expr_lit
+            (Pulse2Rust_Rust_Syntax.Lit_int
+               {
+                 Pulse2Rust_Rust_Syntax.lit_int_val = lit_int_val;
+                 Pulse2Rust_Rust_Syntax.lit_int_signed = lit_int_signed;
+                 Pulse2Rust_Rust_Syntax.lit_int_width = lit_int_width
+               })
+      | FStar_Extraction_ML_Syntax.MLE_Var x ->
+          let uu___ = varname x in Pulse2Rust_Rust_Syntax.Expr_path uu___
+      | FStar_Extraction_ML_Syntax.MLE_Name p ->
+          Pulse2Rust_Rust_Syntax.Expr_path (FStar_Pervasives_Native.snd p)
+      | FStar_Extraction_ML_Syntax.MLE_Let uu___ ->
           let uu___1 =
-            let uu___2 = varname x in Pulse2Rust_Rust_Syntax.Expr_path uu___2 in
-          Pulse2Rust_Rust_Syntax.Stmt_expr uu___1 in
-        [uu___]
-    | FStar_Extraction_ML_Syntax.MLE_Name p ->
-        [Pulse2Rust_Rust_Syntax.Stmt_expr
-           (Pulse2Rust_Rust_Syntax.Expr_path
-              (FStar_Extraction_ML_Syntax.mlpath_to_string p))]
-    | FStar_Extraction_ML_Syntax.MLE_Let
-        ((FStar_Extraction_ML_Syntax.NonRec, lb::[]), e1) ->
-        let is_mut = false in
-        let s =
-          let uu___ = extract_mlexpr lb.FStar_Extraction_ML_Syntax.mllb_def in
-          Pulse2Rust_Rust_Syntax.mk_local_stmt
-            lb.FStar_Extraction_ML_Syntax.mllb_name is_mut uu___ in
-        let uu___ = extract_mlexpr_to_stmts e1 in s :: uu___
-    | uu___ ->
-        let uu___1 =
-          let uu___2 = FStar_Extraction_ML_Syntax.mlexpr_to_string e in
-          FStar_Compiler_Util.format1 "mlexpr_to_stmt  %s" uu___2 in
-        fail_nyi uu___1
+            FStar_Compiler_Effect.op_Bar_Greater e
+              (extract_mlexpr_to_stmts g) in
+          FStar_Compiler_Effect.op_Bar_Greater uu___1
+            Pulse2Rust_Rust_Syntax.mk_block_expr
+      | FStar_Extraction_ML_Syntax.MLE_App
+          ({
+             FStar_Extraction_ML_Syntax.expr =
+               FStar_Extraction_ML_Syntax.MLE_TApp
+               ({
+                  FStar_Extraction_ML_Syntax.expr =
+                    FStar_Extraction_ML_Syntax.MLE_Name p;
+                  FStar_Extraction_ML_Syntax.mlty = uu___;
+                  FStar_Extraction_ML_Syntax.loc = uu___1;_},
+                uu___2::[]);
+             FStar_Extraction_ML_Syntax.mlty = uu___3;
+             FStar_Extraction_ML_Syntax.loc = uu___4;_},
+           e1::e2::uu___5::[])
+          when
+          let uu___6 = FStar_Extraction_ML_Syntax.string_of_mlpath p in
+          uu___6 = "Pulse.Lib.Reference.op_Colon_Equals" ->
+          let e11 = extract_mlexpr g e1 in
+          let e21 = extract_mlexpr g e2 in
+          let uu___6 = type_of g e11 in
+          (match uu___6 with
+           | (uu___7, b) ->
+               if b
+               then Pulse2Rust_Rust_Syntax.mk_assign e11 e21
+               else Pulse2Rust_Rust_Syntax.mk_ref_assign e11 e21)
+      | FStar_Extraction_ML_Syntax.MLE_App
+          ({
+             FStar_Extraction_ML_Syntax.expr =
+               FStar_Extraction_ML_Syntax.MLE_TApp
+               ({
+                  FStar_Extraction_ML_Syntax.expr =
+                    FStar_Extraction_ML_Syntax.MLE_Name p;
+                  FStar_Extraction_ML_Syntax.mlty = uu___;
+                  FStar_Extraction_ML_Syntax.loc = uu___1;_},
+                uu___2::[]);
+             FStar_Extraction_ML_Syntax.mlty = uu___3;
+             FStar_Extraction_ML_Syntax.loc = uu___4;_},
+           e1::uu___5::uu___6::[])
+          when
+          let uu___7 = FStar_Extraction_ML_Syntax.string_of_mlpath p in
+          uu___7 = "Pulse.Lib.Reference.op_Bang" ->
+          let e2 = extract_mlexpr g e1 in
+          let uu___7 = type_of g e2 in
+          (match uu___7 with
+           | (uu___8, b) ->
+               if b then e2 else Pulse2Rust_Rust_Syntax.mk_ref_read e2)
+      | FStar_Extraction_ML_Syntax.MLE_App
+          ({
+             FStar_Extraction_ML_Syntax.expr =
+               FStar_Extraction_ML_Syntax.MLE_Name p;
+             FStar_Extraction_ML_Syntax.mlty = uu___;
+             FStar_Extraction_ML_Syntax.loc = uu___1;_},
+           {
+             FStar_Extraction_ML_Syntax.expr =
+               FStar_Extraction_ML_Syntax.MLE_Fun (uu___2, cond);
+             FStar_Extraction_ML_Syntax.mlty = uu___3;
+             FStar_Extraction_ML_Syntax.loc = uu___4;_}::{
+                                                           FStar_Extraction_ML_Syntax.expr
+                                                             =
+                                                             FStar_Extraction_ML_Syntax.MLE_Fun
+                                                             (uu___5, body);
+                                                           FStar_Extraction_ML_Syntax.mlty
+                                                             = uu___6;
+                                                           FStar_Extraction_ML_Syntax.loc
+                                                             = uu___7;_}::[])
+          when
+          let uu___8 = FStar_Extraction_ML_Syntax.string_of_mlpath p in
+          uu___8 = "Pulse.Lib.Core.while_" ->
+          let expr_while_cond = extract_mlexpr g cond in
+          let expr_while_body = extract_mlexpr_to_stmts g body in
+          Pulse2Rust_Rust_Syntax.Expr_while
+            {
+              Pulse2Rust_Rust_Syntax.expr_while_cond = expr_while_cond;
+              Pulse2Rust_Rust_Syntax.expr_while_body = expr_while_body
+            }
+      | FStar_Extraction_ML_Syntax.MLE_App (head, args) ->
+          let head1 = extract_mlexpr g head in
+          let args1 = FStar_Compiler_List.map (extract_mlexpr g) args in
+          Pulse2Rust_Rust_Syntax.mk_call head1 args1
+      | FStar_Extraction_ML_Syntax.MLE_TApp (head, uu___) ->
+          extract_mlexpr g head
+      | FStar_Extraction_ML_Syntax.MLE_If (cond, if_then, if_else_opt) ->
+          let cond1 = extract_mlexpr g cond in
+          let then_ = extract_mlexpr_to_stmts g if_then in
+          let else_ =
+            FStar_Compiler_Util.map_option (extract_mlexpr g) if_else_opt in
+          let else_1 =
+            match else_ with
+            | FStar_Pervasives_Native.None -> else_
+            | FStar_Pervasives_Native.Some (Pulse2Rust_Rust_Syntax.Expr_if
+                uu___) -> else_
+            | FStar_Pervasives_Native.Some (Pulse2Rust_Rust_Syntax.Expr_block
+                uu___) -> else_
+            | FStar_Pervasives_Native.Some else_2 ->
+                let uu___ =
+                  Pulse2Rust_Rust_Syntax.mk_block_expr
+                    [Pulse2Rust_Rust_Syntax.Stmt_expr else_2] in
+                FStar_Pervasives_Native.Some uu___ in
+          Pulse2Rust_Rust_Syntax.mk_if cond1 then_ else_1
+      | uu___ ->
+          let uu___1 =
+            let uu___2 = FStar_Extraction_ML_Syntax.mlexpr_to_string e in
+            FStar_Compiler_Util.format1 "mlexpr %s" uu___2 in
+          fail_nyi uu___1
+and (extract_mlexpr_to_stmts :
+  env ->
+    FStar_Extraction_ML_Syntax.mlexpr ->
+      Pulse2Rust_Rust_Syntax.stmt Prims.list)
+  =
+  fun g ->
+    fun e ->
+      match e.FStar_Extraction_ML_Syntax.expr with
+      | FStar_Extraction_ML_Syntax.MLE_Const
+          (FStar_Extraction_ML_Syntax.MLC_Unit) -> []
+      | FStar_Extraction_ML_Syntax.MLE_Var x ->
+          let uu___ =
+            let uu___1 =
+              let uu___2 = varname x in
+              Pulse2Rust_Rust_Syntax.Expr_path uu___2 in
+            Pulse2Rust_Rust_Syntax.Stmt_expr uu___1 in
+          [uu___]
+      | FStar_Extraction_ML_Syntax.MLE_Name p ->
+          [Pulse2Rust_Rust_Syntax.Stmt_expr
+             (Pulse2Rust_Rust_Syntax.Expr_path
+                (FStar_Extraction_ML_Syntax.mlpath_to_string p))]
+      | FStar_Extraction_ML_Syntax.MLE_Let
+          ((FStar_Extraction_ML_Syntax.NonRec, lb::[]), e1) ->
+          let is_mut =
+            FStar_Compiler_List.contains FStar_Extraction_ML_Syntax.Mutable
+              lb.FStar_Extraction_ML_Syntax.mllb_meta in
+          let uu___ =
+            if is_mut
+            then
+              let init =
+                match (lb.FStar_Extraction_ML_Syntax.mllb_def).FStar_Extraction_ML_Syntax.expr
+                with
+                | FStar_Extraction_ML_Syntax.MLE_App
+                    ({
+                       FStar_Extraction_ML_Syntax.expr =
+                         FStar_Extraction_ML_Syntax.MLE_Name p;
+                       FStar_Extraction_ML_Syntax.mlty = uu___1;
+                       FStar_Extraction_ML_Syntax.loc = uu___2;_},
+                     init1::[])
+                    when
+                    let uu___3 =
+                      FStar_Extraction_ML_Syntax.string_of_mlpath p in
+                    uu___3 = "Pulse.Lib.Reference.alloc" -> init1
+                | uu___1 ->
+                    let uu___2 =
+                      let uu___3 =
+                        FStar_Extraction_ML_Syntax.mlexpr_to_string
+                          lb.FStar_Extraction_ML_Syntax.mllb_def in
+                      FStar_Compiler_Util.format1
+                        "unexpected initializer for mutable local: %s" uu___3 in
+                    fail uu___2 in
+              let ty =
+                match lb.FStar_Extraction_ML_Syntax.mllb_tysc with
+                | FStar_Pervasives_Native.Some
+                    ([], FStar_Extraction_ML_Syntax.MLTY_Named (ty1::[], p))
+                    when
+                    let uu___1 =
+                      FStar_Extraction_ML_Syntax.string_of_mlpath p in
+                    uu___1 = "Pulse.Lib.Reference.ref" -> ty1
+                | uu___1 ->
+                    let uu___2 =
+                      let uu___3 =
+                        let uu___4 =
+                          FStar_Compiler_Util.must
+                            lb.FStar_Extraction_ML_Syntax.mllb_tysc in
+                        FStar_Extraction_ML_Syntax.mltyscheme_to_string
+                          uu___4 in
+                      FStar_Compiler_Util.format1
+                        "unexpected type of mutable local: %s" uu___3 in
+                    fail uu___2 in
+              (init, ty)
+            else
+              (let uu___2 =
+                 let uu___3 =
+                   FStar_Compiler_Util.must
+                     lb.FStar_Extraction_ML_Syntax.mllb_tysc in
+                 FStar_Pervasives_Native.snd uu___3 in
+               ((lb.FStar_Extraction_ML_Syntax.mllb_def), uu___2)) in
+          (match uu___ with
+           | (init, ty) ->
+               let s =
+                 let uu___1 = extract_mlexpr g init in
+                 Pulse2Rust_Rust_Syntax.mk_local_stmt
+                   lb.FStar_Extraction_ML_Syntax.mllb_name is_mut uu___1 in
+               let uu___1 =
+                 let uu___2 =
+                   let uu___3 = extract_mlty g ty in
+                   push_local g lb.FStar_Extraction_ML_Syntax.mllb_name
+                     uu___3 is_mut in
+                 extract_mlexpr_to_stmts uu___2 e1 in
+               s :: uu___1)
+      | uu___ ->
+          let uu___1 =
+            let uu___2 = FStar_Extraction_ML_Syntax.mlexpr_to_string e in
+            FStar_Compiler_Util.format1 "mlexpr_to_stmt  %s" uu___2 in
+          fail_nyi uu___1
 let (extract_top_level_lb :
-  FStar_Extraction_ML_Syntax.mlletbinding -> Pulse2Rust_Rust_Syntax.fn) =
-  fun lbs ->
-    let uu___ = lbs in
-    match uu___ with
-    | (is_rec, lbs1) ->
-        if is_rec = FStar_Extraction_ML_Syntax.Rec
-        then fail_nyi "recursive let bindings"
-        else
-          (let uu___2 = lbs1 in
-           match uu___2 with
-           | lb::[] ->
-               (if
-                  FStar_Pervasives_Native.uu___is_None
-                    lb.FStar_Extraction_ML_Syntax.mllb_tysc
-                then
-                  (let uu___4 =
-                     FStar_Compiler_Util.format1
-                       "unexpected: mllb_tsc is None for %s"
-                       lb.FStar_Extraction_ML_Syntax.mllb_name in
-                   fail uu___4)
-                else ();
-                (let uu___4 = lb.FStar_Extraction_ML_Syntax.mllb_tysc in
-                 match uu___4 with
-                 | FStar_Pervasives_Native.Some tsc ->
-                     let uu___5 =
-                       match (lb.FStar_Extraction_ML_Syntax.mllb_def).FStar_Extraction_ML_Syntax.expr
-                       with
-                       | FStar_Extraction_ML_Syntax.MLE_Fun (bs, body) ->
-                           let uu___6 =
-                             FStar_Compiler_List.map
-                               FStar_Pervasives_Native.fst bs in
-                           (uu___6, body)
-                       | uu___6 ->
-                           let uu___7 =
-                             let uu___8 =
-                               FStar_Extraction_ML_Syntax.mlexpr_to_string
-                                 lb.FStar_Extraction_ML_Syntax.mllb_def in
-                             FStar_Compiler_Util.format1
-                               "top level lb def %s" uu___8 in
-                           fail_nyi uu___7 in
-                     (match uu___5 with
-                      | (arg_names, body) ->
-                          let uu___6 = arg_ts_and_ret_t tsc in
-                          (match uu___6 with
-                           | (tvars, arg_ts, ret_t) ->
-                               let fn_sig =
+  env ->
+    FStar_Extraction_ML_Syntax.mlletbinding ->
+      (Pulse2Rust_Rust_Syntax.fn * env))
+  =
+  fun g ->
+    fun lbs ->
+      let uu___ = lbs in
+      match uu___ with
+      | (is_rec, lbs1) ->
+          if is_rec = FStar_Extraction_ML_Syntax.Rec
+          then fail_nyi "recursive let bindings"
+          else
+            (let uu___2 = lbs1 in
+             match uu___2 with
+             | lb::[] ->
+                 (if
+                    FStar_Pervasives_Native.uu___is_None
+                      lb.FStar_Extraction_ML_Syntax.mllb_tysc
+                  then
+                    (let uu___4 =
+                       FStar_Compiler_Util.format1
+                         "unexpected: mllb_tsc is None for %s"
+                         lb.FStar_Extraction_ML_Syntax.mllb_name in
+                     fail uu___4)
+                  else ();
+                  (let uu___4 = lb.FStar_Extraction_ML_Syntax.mllb_tysc in
+                   match uu___4 with
+                   | FStar_Pervasives_Native.Some tsc ->
+                       let uu___5 =
+                         match (lb.FStar_Extraction_ML_Syntax.mllb_def).FStar_Extraction_ML_Syntax.expr
+                         with
+                         | FStar_Extraction_ML_Syntax.MLE_Fun (bs, body) ->
+                             let uu___6 =
+                               FStar_Compiler_List.map
+                                 FStar_Pervasives_Native.fst bs in
+                             (uu___6, body)
+                         | uu___6 ->
+                             let uu___7 =
+                               let uu___8 =
+                                 FStar_Extraction_ML_Syntax.mlexpr_to_string
+                                   lb.FStar_Extraction_ML_Syntax.mllb_def in
+                               FStar_Compiler_Util.format1
+                                 "top level lb def %s" uu___8 in
+                             fail_nyi uu___7 in
+                       (match uu___5 with
+                        | (arg_names, body) ->
+                            let uu___6 = arg_ts_and_ret_t tsc in
+                            (match uu___6 with
+                             | (tvars, arg_ts, ret_t) ->
                                  let uu___7 =
-                                   FStar_Compiler_List.map tyvar_of tvars in
-                                 extract_top_level_sig
-                                   lb.FStar_Extraction_ML_Syntax.mllb_name
-                                   uu___7 arg_names arg_ts ret_t in
-                               let fn_body = extract_mlexpr_to_stmts body in
-                               Pulse2Rust_Rust_Syntax.mk_fn fn_sig fn_body)))))
+                                   let uu___8 =
+                                     FStar_Compiler_List.map tyvar_of tvars in
+                                   extract_top_level_sig g
+                                     lb.FStar_Extraction_ML_Syntax.mllb_name
+                                     uu___8 arg_names arg_ts ret_t in
+                                 (match uu___7 with
+                                  | (fn_sig, g_body) ->
+                                      let fn_body =
+                                        extract_mlexpr_to_stmts g_body body in
+                                      let uu___8 =
+                                        Pulse2Rust_Rust_Syntax.mk_fn fn_sig
+                                          fn_body in
+                                      let uu___9 =
+                                        push_fv g
+                                          lb.FStar_Extraction_ML_Syntax.mllb_name
+                                          fn_sig in
+                                      (uu___8, uu___9)))))))
 let (extract_one : Prims.string -> unit) =
   fun file ->
     let uu___ =
@@ -372,21 +570,27 @@ let (extract_one : Prims.string -> unit) =
     match uu___ with
     | (gamma, decls) ->
         let uu___1 = uu___ in
-        FStar_Compiler_List.iter
-          (fun d ->
-             match d with
-             | FStar_Extraction_ML_Syntax.MLM_Let lb ->
-                 let f = extract_top_level_lb lb in
-                 (FStar_Compiler_Util.print_string "Extracted to:\n";
-                  (let uu___3 =
-                     let uu___4 = RustBindings.fn_to_string f in
-                     Prims.op_Hat uu___4 "\n" in
-                   FStar_Compiler_Util.print_string uu___3))
-             | uu___2 ->
-                 let uu___3 =
-                   let uu___4 =
-                     FStar_Extraction_ML_Syntax.mlmodule1_to_string d in
-                   FStar_Compiler_Util.format1 "top level decl %s" uu___4 in
-                 fail_nyi uu___3) decls
+        let uu___2 =
+          FStar_Compiler_List.fold_left
+            (fun g ->
+               fun d ->
+                 match d with
+                 | FStar_Extraction_ML_Syntax.MLM_Let lb ->
+                     let uu___3 = extract_top_level_lb g lb in
+                     (match uu___3 with
+                      | (f, g1) ->
+                          (FStar_Compiler_Util.print_string "Extracted to:\n";
+                           (let uu___6 =
+                              let uu___7 = RustBindings.fn_to_rust f in
+                              Prims.op_Hat uu___7 "\n" in
+                            FStar_Compiler_Util.print_string uu___6);
+                           g1))
+                 | uu___3 ->
+                     let uu___4 =
+                       let uu___5 =
+                         FStar_Extraction_ML_Syntax.mlmodule1_to_string d in
+                       FStar_Compiler_Util.format1 "top level decl %s" uu___5 in
+                     fail_nyi uu___4) (empty_env ()) decls in
+        ()
 let (extract : Prims.string Prims.list -> unit) =
   fun files -> FStar_Compiler_List.iter extract_one files
